Prove expansion for alpha equiv
In particular, prove that we can add identity map to both sides
under mild conditions
Generalizes several existing lemmas
Used to prove congruences for terms with binders
Only remaining part before conversion is transitivity
Defined aunion and refactored

proofs/core/Alpha.v
@@ -1625,6 +1625,15 @@ Proof.
     intros; destruct_all; subst; try discriminate; contradiction.
 Qed.
 
+(*TODO: use*)
+Definition aunion {A B: Type} `{countable.Countable A} (m1 m2: amap A B) : amap A B :=
+  amap_union (fun u _ => Some u) m1 m2.
+
+Lemma aunion_lookup {A B: Type} `{countable.Countable A} (m1 m2: amap A B) x:
+  amap_lookup (aunion m1 m2) x =
+  match amap_lookup m1 x with | Some y => Some y | None => amap_lookup m2 x end.
+Proof. apply amap_union_lookup. Qed.
+
 (*Check for alpha equivalence*)
 (*NOTE: we use the more general version of [a_equiv_p]: this is OK for semantics and typing
   and it has much nicer syntactic properties*)
@@ -1656,7 +1665,7 @@ Fixpoint alpha_equiv_t (m1 m2: amap vsymbol vsymbol) (t1 t2: term) : bool :=
     all2 (fun (x1 x2: pattern * term) =>
       match (a_equiv_p (fst x1) (fst x2)) with
       | Some (pm1, pm2) => alpha_equiv_t 
-          (amap_union (fun x _ => Some x) pm1 m1) (amap_union (fun x _ => Some x) pm2 m2) (snd x1) (snd x2)
+          (aunion pm1 m1) (aunion pm2 m2) (snd x1) (snd x2)
       | None => false
       end) ps1 ps2
   | Teps f1 x, Teps f2 y => 
@@ -1702,7 +1711,7 @@ with alpha_equiv_f (m1 m2: amap vsymbol vsymbol) (f1 f2: formula) {struct f1} : 
     all2 (fun (x1 x2: pattern * formula) =>
       match (a_equiv_p (fst x1) (fst x2)) with
       | Some (pm1, pm2) => alpha_equiv_f 
-          (amap_union (fun x _ => Some x) pm1 m1) (amap_union (fun x _ => Some x) pm2 m2) (snd x1) (snd x2)
+          (aunion pm1 m1) (aunion pm2 m2) (snd x1) (snd x2)
       | None => false
       end) ps1 ps2
   | _, _ => false
@@ -1848,7 +1857,7 @@ Proof.
       inversion Hps; subst. eapply H1; eauto.
       * (*Separate lemma?*)
         intros x y Heq Hlookup1 Hlookup2.
-        rewrite amap_union_lookup in Hlookup1, Hlookup2.
+        rewrite aunion_lookup in Hlookup1, Hlookup2.
         (*NOTE: need to use free vars and bij information*)
         assert (Hbij:=a_equiv_p_bij Halphap).
         destruct (amap_lookup pm1 x) as [y1|] eqn : Hlook1; [inversion Hlookup1; subst |].
@@ -1882,7 +1891,7 @@ Proof.
             ** apply Hfvp2y in C; rewrite amap_mem_spec, Hlook2 in C. discriminate.
             ** apply Hfvp1x in C; rewrite amap_mem_spec, Hlook1 in C. discriminate.
       * (*None case*)
-        intros x. rewrite !amap_union_lookup.
+        intros x. rewrite !aunion_lookup.
         destruct (amap_lookup pm1 x) eqn : Hlook1; [discriminate|].
         destruct (amap_lookup pm2 x) eqn : Hlook2; [discriminate|].
         intros Hlookup1 Hlookup2.
@@ -2047,7 +2056,7 @@ Proof.
     + (*Reason about [extend_val_with_list]*)
       inversion Hps; subst. eapply H1; eauto.
       * intros x y Heq Hlookup1 Hlookup2.
-        rewrite amap_union_lookup in Hlookup1, Hlookup2.
+        rewrite aunion_lookup in Hlookup1, Hlookup2.
         assert (Hbij:=a_equiv_p_bij Halphap).
         destruct (amap_lookup pm1 x) as [y1|] eqn : Hlook1; [inversion Hlookup1; subst |].
         -- (*Now know x in fv p1 and y is in fv p2, so x is in a1*)
@@ -2079,7 +2088,7 @@ Proof.
             ** apply Hfvp2y in C; rewrite amap_mem_spec, Hlook2 in C. discriminate.
             ** apply Hfvp1x in C; rewrite amap_mem_spec, Hlook1 in C. discriminate.
       * (*None case*)
-        intros x. rewrite !amap_union_lookup.
+        intros x. rewrite !aunion_lookup.
         destruct (amap_lookup pm1 x) eqn : Hlook1; [discriminate|].
         destruct (amap_lookup pm2 x) eqn : Hlook2; [discriminate|].
         intros Hlookup1 Hlookup2.
@@ -5134,7 +5143,7 @@ Proof.
     inversion H0; subst. 
     destruct a. bool_to_prop; split_all; auto.
     simpl. rewrite a_equiv_p_refl.
-    apply H2. intros x y. rewrite amap_union_lookup.
+    apply H2. intros x y. rewrite aunion_lookup.
     destruct (amap_lookup _ x) as [y1|] eqn : Hget; auto.
     apply id_map_id in Hget. subst. intros Hsome; inversion Hsome; subst; auto.
   - bool_to_prop; split; [simpl_sumbool | apply H]; auto;
@@ -5158,7 +5167,7 @@ Proof.
     inversion H0; subst. 
     destruct a. bool_to_prop; split_all; auto.
     simpl. rewrite a_equiv_p_refl.
-    apply H2. intros x y. rewrite amap_union_lookup.
+    apply H2. intros x y. rewrite aunion_lookup.
     destruct (amap_lookup _ x) as [y1|] eqn : Hget; auto.
     apply id_map_id in Hget. subst. intros Hsome; inversion Hsome; subst; auto.
 Qed.
@@ -5934,7 +5943,7 @@ Proof.
         rewrite Forall_forall in IH2. eapply IH2; eauto.
         + apply in_map. auto.
         + (*Map preservation*)
-          intros x y Hlookup. rewrite amap_union_lookup in Hlookup.
+          intros x y Hlookup. rewrite aunion_lookup in Hlookup.
           destruct (amap_lookup res1 x) as [y1|] eqn : Hlook1; auto.
           inversion Hlookup; subst.
           (*Use pattern types result*)
@@ -6034,7 +6043,7 @@ Proof.
         rewrite Forall_forall in IH2. eapply IH2; eauto.
         + apply in_map. auto.
         + (*Map preservation*)
-          intros x y Hlookup. rewrite amap_union_lookup in Hlookup.
+          intros x y Hlookup. rewrite aunion_lookup in Hlookup.
           destruct (amap_lookup res1 x) as [y1|] eqn : Hlook1; auto.
           inversion Hlookup; subst.
           (*Use pattern types result*)
@@ -6178,6 +6187,11 @@ Proof.
   - rewrite amap_set_lookup_diff by auto. reflexivity.
 Qed.
 
+(*TODO: move*)
+Lemma amap_mem_aunion_some {A B: Type} `{countable.Countable A} (m1 m2: amap A B) x:
+  amap_mem x (aunion m1 m2) = amap_mem x m1 || amap_mem x m2.
+Proof. apply amap_mem_union_some; auto. Qed.
+
 Lemma alpha_fv_filter t1 f1:
   (forall t2 m1 m2 (Heq: alpha_equiv_t m1 m2 t1 t2),
     aset_filter (fun x => negb (amap_mem x m1)) (tm_fv t1) =
@@ -6253,12 +6267,12 @@ Proof.
     destruct Halphap as [Hmemres1 Hmemres2].
     prove_filter_eq.
     (*NOTE: both proofs will be the same, should factor out*)
-    + intros x. rewrite amap_mem_union_some by auto.
+    + intros x. rewrite amap_mem_aunion_some.
       rewrite negb_orb. f_equal. f_equal.
       destruct (aset_mem_dec _ _) as [Hmem | Hmem]; simpl; auto;
       rewrite <- Hmemres1 in Hmem; auto.
       destruct (amap_mem _ _); auto. exfalso; apply Hmem; auto.
-    + intros x. rewrite amap_mem_union_some by auto.
+    + intros x. rewrite amap_mem_aunion_some by auto.
       rewrite negb_orb. f_equal. f_equal.
       destruct (aset_mem_dec _ _) as [Hmem | Hmem]; simpl; auto;
       rewrite <- Hmemres2 in Hmem; auto.
@@ -6335,12 +6349,12 @@ Proof.
     destruct Halphap as [Hmemres1 Hmemres2].
     prove_filter_eq.
     (*NOTE: both proofs will be the same, should factor out*)
-    + intros x. rewrite amap_mem_union_some by auto.
+    + intros x. rewrite amap_mem_aunion_some by auto.
       rewrite negb_orb. f_equal. f_equal.
       destruct (aset_mem_dec _ _) as [Hmem | Hmem]; simpl; auto;
       rewrite <- Hmemres1 in Hmem; auto.
       destruct (amap_mem _ _); auto. exfalso; apply Hmem; auto.
-    + intros x. rewrite amap_mem_union_some by auto.
+    + intros x. rewrite amap_mem_aunion_some by auto.
       rewrite negb_orb. f_equal. f_equal.
       destruct (aset_mem_dec _ _) as [Hmem | Hmem]; simpl; auto;
       rewrite <- Hmemres2 in Hmem; auto.
@@ -6569,30 +6583,30 @@ Proof.
       rewrite amap_set_lookup_diff; auto.
 Qed.
 
-Lemma amap_union_remove_infst {A B: Type} `{countable.Countable A} (m1 m2: amap A B) (x1: A) :
+Lemma aunion_remove_infst {A B: Type} `{countable.Countable A} (m1 m2: amap A B) (x1: A) :
   amap_mem x1 m1 ->
-  amap_union (fun z _ => Some z) m1 (amap_remove _ _ x1 m2) = amap_union (fun z _ => Some z) m1 m2.
+  aunion m1 (amap_remove _ _ x1 m2) = aunion m1 m2.
 Proof.
   rewrite amap_mem_spec. intros Hmem.
   apply amap_ext. intros x.
-  rewrite !amap_union_lookup.
+  rewrite !aunion_lookup.
   destruct (EqDecision0 x x1); subst.
   - rewrite amap_remove_same; auto. destruct (amap_lookup m1 x1); auto. discriminate.
   - rewrite amap_remove_diff; auto.
 Qed.
 
 (*TODO: what is theorem we need: we can bring remove to front of union?*)
-Lemma amap_union_remove_not_infst {A B: Type} `{countable.Countable A} (m1 m2: amap A B) (x1: A) :
+Lemma aunion_remove_not_infst {A B: Type} `{countable.Countable A} (m1 m2: amap A B) (x1: A) :
   ~ amap_mem x1 m1 ->
-  amap_union (fun z _ => Some z) m1 (amap_remove _ _ x1 m2) = 
-  amap_remove _ _ x1 (amap_union (fun z _ => Some z) m1 m2).
+  aunion  m1 (amap_remove _ _ x1 m2) = 
+  amap_remove _ _ x1 (aunion m1 m2).
 Proof.
   rewrite amap_mem_spec. intros Hmem.
   apply amap_ext. intros x.
-  rewrite !amap_union_lookup.
+  rewrite !aunion_lookup.
   destruct (EqDecision0 x x1); subst.
   - rewrite !amap_remove_same. destruct (amap_lookup m1 x1); auto. exfalso; apply Hmem; auto.
-  - rewrite !amap_remove_diff; auto. rewrite !amap_union_lookup. auto.
+  - rewrite !amap_remove_diff; auto. rewrite !aunion_lookup. auto.
 Qed.
 
 (*NOTE: can I just prove that we can remove it from the second map?*)
@@ -6648,10 +6662,10 @@ Proof.
     apply a_equiv_p_vars_iff in Halphap. destruct Halphap as [Hiff1 Hiff2].
     destruct (aset_mem_dec y2 (pat_fv p2)) as [Hinfv | Hnotinfv].
     + (*Get rid of remove because in first anyway*)
-      rewrite amap_union_remove_infst by (rewrite Hiff2; auto).
+      rewrite aunion_remove_infst by (rewrite Hiff2; auto).
       reflexivity.
     + (*Here, we can bring to front because not in first*)
-      rewrite amap_union_remove_not_infst by (rewrite Hiff2; auto).
+      rewrite aunion_remove_not_infst by (rewrite Hiff2; auto).
       apply IH1; auto.
   - (*Teps*)
     destruct t2 as [| | | | | | f2 x2]; auto. simpl in Hfree. simpl_set. f_equal; auto.
@@ -6707,9 +6721,9 @@ Proof.
     destruct (a_equiv_p p1 p2) as [[res1 res2]|] eqn : Halphap; auto.
     apply a_equiv_p_vars_iff in Halphap. destruct Halphap as [Hiff1 Hiff2].
     destruct (aset_mem_dec y2 (pat_fv p2)) as [Hinfv | Hnotinfv].
-    + rewrite amap_union_remove_infst by (rewrite Hiff2; auto).
+    + rewrite aunion_remove_infst by (rewrite Hiff2; auto).
       reflexivity.
-    + rewrite amap_union_remove_not_infst by (rewrite Hiff2; auto).
+    + rewrite aunion_remove_not_infst by (rewrite Hiff2; auto).
       apply IH1; auto.
 Qed.
 
@@ -6972,7 +6986,330 @@ Qed.
 
 Definition alpha_equiv_t_redundant t := proj_tm alpha_equiv_redundant t.
 Definition alpha_equiv_f_redundant f := proj_fmla alpha_equiv_redundant f.
+*)
 
+(*We prove we can always add bindings (x, x) to the map if all are not in there already*)
+
+Definition mk_id_map {A: Type} `{countable.Countable A} (s: aset A): amap A A :=
+  fold_right (fun x acc => amap_set acc x x) amap_empty (aset_to_list s).
+
+Lemma mk_id_map_lookup {A: Type} `{countable.Countable A} (s: aset A) x y:
+  amap_lookup (mk_id_map s) x = Some y <-> x = y /\ aset_mem x s.
+Proof.
+  unfold mk_id_map. rewrite <- aset_to_list_in.
+  induction (aset_to_list) as [| h t IH]; simpl; auto.
+  - rewrite amap_empty_get. split; [discriminate| intros; destruct_all; contradiction].
+  - destruct (EqDecision0 x h); subst.
+    + rewrite amap_set_lookup_same. split; intros Hsome; destruct_all; auto. inversion Hsome; auto.
+    + rewrite amap_set_lookup_diff by auto. rewrite IH. split; intros; destruct_all; auto. contradiction.
+Qed.
+
+Lemma mk_id_map_lookup_none {A: Type} `{countable.Countable A} (s: aset A) x:
+  amap_lookup (mk_id_map s) x = None <-> ~ aset_mem x s.
+Proof.
+  pose proof (mk_id_map_lookup s x x) as Hlook.
+  assert (Hsimpl: x = x /\ aset_mem x s <-> aset_mem x s) by (split; intros; destruct_all; auto).
+  rewrite Hsimpl in Hlook; clear Hsimpl. rewrite <- Hlook.
+  split; intros Hlookup.
+  - rewrite Hlookup. auto.
+  - destruct (amap_lookup (mk_id_map s) x) as [y|] eqn : Hget; auto.
+    apply mk_id_map_lookup in Hget. destruct Hget; subst; contradiction.
+Qed.
+
+(*NOTE: let's see if easier to prove for 1, then extend*)
+
+
+
+Lemma amap_set_aunion_fst  {A B: Type} `{countable.Countable A} (m1 m2: amap A B) x y:
+  amap_set (aunion m1 m2) x y = aunion (amap_set m1 x y) m2.
+Proof.
+  apply amap_ext. intros z. rewrite aunion_lookup.
+  destruct (EqDecision0 x z); subst.
+  - rewrite !amap_set_lookup_same; auto.
+  - rewrite !amap_set_lookup_diff by auto. rewrite aunion_lookup; auto.
+Qed.
+
+Lemma amap_union_assoc  {A B: Type} `{countable.Countable A} (m1 m2 m3: amap A B):
+  aunion m1 (aunion m2 m3) = aunion (aunion m1 m2) m3.
+Proof.
+  apply amap_ext. intros x. rewrite !aunion_lookup.
+  destruct (amap_lookup m1 x); auto.
+Qed.
+
+(*NOTE: if needed, assume no equal elements here - could always move to other set*)
+(*TODO: bad name*)
+Lemma bij_set {A: Type} `{countable.Countable A} (m1 m2: amap A A) x1 y1
+  (Hbij: forall x, amap_lookup m1 x = Some x -> amap_mem x m2):
+  forall x, amap_lookup (amap_set m1 x1 y1) x = Some x -> amap_mem x (amap_set m2 y1 x1).
+Proof.
+  intros x.
+  destruct (EqDecision0 x x1); subst.
+  - rewrite amap_set_lookup_same. intros Hsome; inversion Hsome; auto. subst.
+    rewrite amap_mem_spec, amap_set_lookup_same. auto.
+  - rewrite amap_set_lookup_diff by auto. intros Hlookup.
+    rewrite amap_mem_spec. apply Hbij in Hlookup. rewrite amap_mem_spec in Hlookup.
+    destruct (EqDecision0 x y1); subst.
+    + rewrite amap_set_lookup_same. auto.
+    + rewrite amap_set_lookup_diff by auto. assumption.
+Qed.
+
+(*bij_map implies this condition*)
+Lemma bij_map_cond r1 r2
+  (Hbij: bij_map r1 r2):
+  forall x, amap_lookup r1 x = Some x -> amap_mem x r2.
+Proof.
+  intros x. unfold bij_map in Hbij. rewrite Hbij. rewrite amap_mem_spec.
+  intros Hlook; rewrite Hlook. auto.
+Qed.
+
+Lemma bij_aunion {A: Type} `{countable.Countable A} (r1 r2 m1 m2: amap A A)
+  (Hbij: forall x, amap_lookup m1 x = Some x -> amap_mem x m2)
+  (Hr: forall x, amap_lookup r1 x = Some x -> amap_mem x r2):
+  forall x, amap_lookup (aunion r1 m1) x = Some x -> amap_mem x (aunion r2 m2).
+Proof.
+  intros x. rewrite amap_mem_spec, !aunion_lookup.
+  destruct (amap_lookup r1 x) as [y1|] eqn : Hget1.
+  - intros Hsome; inversion Hsome; subst. apply Hr in Hget1.
+    rewrite amap_mem_spec in Hget1. destruct (amap_lookup r2 x); auto.
+  - intros Hlook. apply Hbij in Hlook.
+    rewrite amap_mem_spec in Hlook. destruct (amap_lookup m2 x); auto.
+    destruct (amap_lookup r2 x); auto.
+Qed.
+
+
+(*We want to prove that if we have a_equiv_t, then we can add bindings (x, x) and
+  still remain alpha equivalent. For generality and induction, we prove the 
+  following lemma: we can always add identical bindings as long as they do not
+  appear later in the map (since we use an order-sensitive union, the order matters).
+  We need a somewhat strange condition that if (x, x) is occurs before 
+  the added set, then x is also in the corresponding other map.
+  We cannot prove the "obvious" condition that the two maps are mirror images:
+  a binding may be replaced in one map but not the other. This weaker condition is
+  enough for us, however.*)
+(*NOTE: could restrict Hm1 and Hm2 to only be true for vars in s, not sure it matters*)
+Lemma alpha_equiv_redundant (s: aset vsymbol) (m3 m4: amap vsymbol vsymbol) 
+  (Hnotin1: forall x, aset_mem x s -> amap_lookup m3 x = None) 
+  (Hnotin2: forall x, aset_mem x s -> amap_lookup m4 x = None)  (t1: term) (f1: formula):
+  (forall (t2: term) (m1 m2: amap vsymbol vsymbol) 
+    (Hm1: forall x, amap_lookup m1 x = Some x -> amap_mem x m2)
+    (Hm2: forall x, amap_lookup m2 x = Some x -> amap_mem x m1),
+    alpha_equiv_t (aunion m1 (aunion (mk_id_map s) m3)) (aunion m2 (aunion (mk_id_map s) m4)) t1 t2 =
+    alpha_equiv_t (aunion m1 m3) (aunion m2 m4) t1 t2) /\
+  (forall (f2: formula) (m1 m2: amap vsymbol vsymbol) 
+    (Hm1: forall x, amap_lookup m1 x = Some x -> amap_mem x m2)
+    (Hm2: forall x, amap_lookup m2 x = Some x -> amap_mem x m1),
+    alpha_equiv_f (aunion m1 (aunion (mk_id_map s) m3)) (aunion m2 (aunion (mk_id_map s) m4)) f1 f2 =
+    alpha_equiv_f (aunion m1 m3) (aunion m2 m4) f1 f2). 
+Proof.
+  revert t1 f1; apply term_formula_ind; intros; auto.
+  - (*Tvar*) destruct t2 as [|v1 | | | | |]; auto. simpl. 
+    unfold alpha_equiv_var.
+    rewrite !aunion_lookup.
+    (*Lots of cases*)
+    destruct (amap_lookup m1 v) as [y1|] eqn : Hget1.
+    + destruct (amap_lookup m2 v1) as [y2|] eqn : Hget2; auto.
+      destruct (amap_lookup (mk_id_map s) v1) as [y3|] eqn : Hget3; auto.
+      apply mk_id_map_lookup in Hget3. destruct_all; subst.
+      vsym_eq y3 y1; simpl; [| destruct (amap_lookup m4 y3); auto].
+      (*know y1 notin m4 by assumption*)
+      rewrite (Hnotin2 y1) by auto. vsym_eq v y1.
+      apply Hm1 in Hget1. rewrite amap_mem_spec, Hget2 in Hget1. discriminate.
+    + (*Now see if v is in s*)
+      destruct (amap_lookup (mk_id_map s) v) as [t|] eqn : Htemp.
+      * rewrite mk_id_map_lookup in Htemp. destruct Htemp as [Ht Hmems]; subst t.
+        rewrite (Hnotin1 v) by auto.
+        destruct (amap_lookup m2 v1) as [y2|] eqn : Hget2.
+        -- vsym_eq v1 v. vsym_eq v y2. apply Hm2 in Hget2. 
+          rewrite amap_mem_spec, Hget1 in Hget2; discriminate.
+        -- destruct (amap_lookup (mk_id_map s) v1) as [t|] eqn : Htemp.
+          ++ rewrite mk_id_map_lookup in Htemp. destruct Htemp as [Heq Hmems']; subst t.
+             rewrite (Hnotin2 v1) by auto. vsym_eq v1 v. vsym_eq v v1.
+          ++ rewrite mk_id_map_lookup_none in Htemp. vsym_eq v1 v. simpl. vsym_eq v v1.
+      * rewrite mk_id_map_lookup_none in Htemp.
+        (*Now know v not in m1 or s*)
+        destruct (amap_lookup m3 v) as [y3|] eqn : Hget3.
+        -- destruct (amap_lookup m2 v1) as [y2|] eqn : Hget2; auto.
+          destruct (amap_lookup (mk_id_map s) v1) as [t|] eqn : Hv1s; auto.
+          rewrite mk_id_map_lookup in Hv1s. destruct Hv1s as [Ht Hmems]; subst t.
+          rewrite (Hnotin2 v1) by auto. vsym_eq v v1. simpl. apply andb_false_r.
+        -- destruct (amap_lookup m2 v1) as [y2|] eqn : Hget2; auto.
+          destruct (amap_lookup (mk_id_map s) v1) as [t|] eqn : Hv1s; auto.
+          rewrite mk_id_map_lookup in Hv1s. destruct Hv1s as [Ht Hmems]; subst t.
+          rewrite (Hnotin2 v1) by auto. vsym_eq v v1.
+  - destruct t2 as [| | f2 tys2 tms2 | | | |]; auto.
+    rename l into tys1; rename l1 into tms1; rename H into IH. simpl.
+    destruct (funsym_eq_dec _ _); subst; auto.
+    simpl in *. destruct (Nat.eqb_spec (length tms1) (length tms2)) as [Hlen|]; auto.
+    destruct (list_eq_dec _ _ _); subst; auto. simpl.
+    generalize dependent tms2. induction tms1 as [| t1 tms1 IHtms]; intros [| t2 tms2]; try discriminate; auto.
+    simpl_set_small. simpl. rewrite !all2_cons. intros Hlen.
+    inversion IH as [| ? ? IH1 IH2]; subst. f_equal; auto.
+  - (*Tlet*) destruct t2 as [| | | tm3 v2 tm4 | | |]; auto. simpl.
+    f_equal; [f_equal|]; auto.
+    rewrite !amap_set_aunion_fst.
+    apply H0; auto; apply bij_set; auto.
+  - (*Tif*) destruct t0; auto. simpl. repeat(f_equal; auto).
+  - (*Tmatch*)
+    destruct t2 as [ | | | | | tm2 ty2 ps2 |]; auto.
+    rename tm into tm1; rename v into ty1; rename ps into ps1; rename H into IH1; rename H0 into IHps.
+    simpl. rewrite IH1 by auto.
+    destruct (Nat.eqb_spec (length ps1) (length ps2)) as [Hlen |].
+    2: { rewrite !andb_false_r; auto. }
+    f_equal.
+    clear IH1. generalize dependent ps2.
+    induction ps1 as [| [p1 t1] ps1 IHps1]; intros [| [p2 t2] ps2]; try discriminate; auto.
+    simpl. rewrite !all2_cons.
+    intros Hlen. simpl.
+    inversion IHps as [|? ? IH1 IH2]; subst.
+    rewrite IHps1 by auto. f_equal.
+    destruct (a_equiv_p p1 p2) as [[res1 res2]|] eqn : Halphap; auto.
+    rewrite !(amap_union_assoc res1), !(amap_union_assoc res2).
+    apply IH1. 
+    + apply bij_aunion; auto. apply bij_map_cond. apply a_equiv_p_bij in Halphap; auto.
+    + apply bij_aunion; auto. apply bij_map_cond. apply a_equiv_p_bij in Halphap.
+      rewrite bij_map_sym in Halphap. auto.
+  - (*Teps*)
+    destruct t2 as [| | | | | | f2 x2]; auto. simpl. f_equal; auto.
+    rewrite !amap_set_aunion_fst. apply H; auto; apply bij_set; auto.
+  - (*Fpred*)
+    destruct f2 as [p2 tys2 tms2 | | | | | | | | |]; auto.
+    rename tms into tms1; rename H into IH. simpl.
+    destruct (predsym_eq_dec _ _); subst; auto.
+    simpl in *. destruct (Nat.eqb_spec (length tms1) (length tms2)) as [Hlen|]; auto.
+    destruct (list_eq_dec _ _ _); subst; auto. simpl.
+    generalize dependent tms2. induction tms1 as [| t1 tms1 IHtms]; intros [| t2 tms2]; try discriminate; auto.
+    simpl_set_small. simpl. rewrite !all2_cons. intros Hlen.
+    inversion IH as [| ? ? IH1 IH2]; subst. f_equal; auto.
+  - (*Fquant*)
+    destruct f2 as [ | q2 x2 f2 | | | | | | | |]; auto. simpl.
+    f_equal. rewrite !amap_set_aunion_fst. apply H; auto; apply bij_set; auto.
+  - (*Feq*) destruct f2; auto; simpl. repeat(f_equal; auto).
+  - (*Fbinop*) destruct f0; auto; simpl. repeat(f_equal; auto).
+  - (*Fnot*) destruct f2; simpl; auto.
+  - (*Flet*) destruct f2 as [ | | | | | | | tm2 v2 f2 | |]; auto; simpl.
+    f_equal; [f_equal|]; auto.
+    rewrite !amap_set_aunion_fst.
+    apply H0; auto; apply bij_set; auto.
+  - (*Fif*) destruct f0; auto; simpl. repeat(f_equal; auto).
+  - (*Fmatch*)
+    destruct f2 as [| | | | | | | | | tm2 ty2 ps2]; auto.
+    rename tm into tm1; rename v into ty1; rename ps into ps1; rename H into IH1; rename H0 into IHps.
+    simpl. rewrite IH1 by auto.
+    destruct (Nat.eqb_spec (length ps1) (length ps2)) as [Hlen |].
+    2: { rewrite !andb_false_r; auto. }
+    f_equal.
+    clear IH1. generalize dependent ps2.
+    induction ps1 as [| [p1 t1] ps1 IHps1]; intros [| [p2 t2] ps2]; try discriminate; auto.
+    simpl. rewrite !all2_cons.
+    intros Hlen. simpl.
+    inversion IHps as [|? ? IH1 IH2]; subst.
+    rewrite IHps1 by auto. f_equal.
+    destruct (a_equiv_p p1 p2) as [[res1 res2]|] eqn : Halphap; auto.
+    rewrite !(amap_union_assoc res1), !(amap_union_assoc res2).
+    apply IH1. 
+    + apply bij_aunion; auto. apply bij_map_cond. apply a_equiv_p_bij in Halphap; auto.
+    + apply bij_aunion; auto. apply bij_map_cond. apply a_equiv_p_bij in Halphap.
+      rewrite bij_map_sym in Halphap. auto.
+Qed.
+
+(*Corollaries*)
+Definition alpha_equiv_t_redundant s m1 m2 m3 m4 Hnotin1 Hnotin2 Hm1 Hm2 t1 t2 :=
+  proj_tm (alpha_equiv_redundant s m3 m4 Hnotin1 Hnotin2) t1 t2 m1 m2 Hm1 Hm2.
+Definition alpha_equiv_f_redundant s m1 m2 m3 m4 Hnotin1 Hnotin2 Hm1 Hm2 f1 f2 :=
+  proj_fmla (alpha_equiv_redundant s m3 m4 Hnotin1 Hnotin2) f1 f2 m1 m2 Hm1 Hm2.
+
+
+(*TODO: see if we need other corollaries, will need one for pattern match*)
+(*TODO: is it easier to do in terms of [mk_id_map] or with m1 and m2 such that they are id maps
+  over the same keyset?*)
+Corollary a_equiv_t_expand (s: aset vsymbol) (t1 t2: term):
+  a_equiv_t t1 t2 = alpha_equiv_t (mk_id_map s) (mk_id_map s) t1 t2.
+Proof.
+  replace (mk_id_map s) with (aunion amap_empty (aunion (mk_id_map s) amap_empty)).
+  2: { unfold aunion; rewrite amap_union_empty_l, amap_union_empty_r. reflexivity. }
+  symmetry.
+  rewrite alpha_equiv_t_redundant; auto; intros x; rewrite amap_empty_get; discriminate.
+Qed.
+
+Corollary a_equiv_f_expand (s: aset vsymbol) (f1 f2: formula):
+  a_equiv_f f1 f2 = alpha_equiv_f (mk_id_map s) (mk_id_map s) f1 f2.
+Proof.
+  replace (mk_id_map s) with (aunion amap_empty (aunion (mk_id_map s) amap_empty)).
+  2: { unfold aunion; rewrite amap_union_empty_l, amap_union_empty_r. reflexivity. }
+  symmetry.
+  rewrite alpha_equiv_f_redundant; auto; intros x; rewrite amap_empty_get; discriminate.
+Qed.
+
+(*And the single versions*)
+
+Lemma mk_id_singleton {A: Type} `{countable.Countable A} (x: A):
+  mk_id_map (aset_singleton x) = amap_singleton x x.
+Proof.
+  apply amap_ext. intros y. unfold amap_singleton.
+  destruct (EqDecision0 x y); subst.
+  - rewrite amap_set_lookup_same. apply mk_id_map_lookup. split; simpl_set; auto.
+  - rewrite amap_set_lookup_diff by auto. rewrite amap_empty_get.
+    apply mk_id_map_lookup_none. simpl_set. auto.
+Qed.
+
+Corollary a_equiv_t_expand_single (x: vsymbol) (t1 t2: term):
+  a_equiv_t t1 t2 = alpha_equiv_t (amap_singleton x x) (amap_singleton x x) t1 t2.
+Proof.
+  rewrite a_equiv_t_expand with (s:=aset_singleton x).
+  rewrite mk_id_singleton. reflexivity.
+Qed.
+
+Corollary a_equiv_f_expand_single (x: vsymbol) (f1 f2: formula):
+  a_equiv_f f1 f2 = alpha_equiv_f (amap_singleton x x) (amap_singleton x x) f1 f2.
+Proof.
+  rewrite a_equiv_f_expand with (s:=aset_singleton x).
+  rewrite mk_id_singleton. reflexivity.
+Qed.
+  
+(*
+
+
+Corollary a_equiv_t_expand (vars: list (vsymbol * vsymbol)) t1 t2:
+  a_equiv_t t1 t2 ->
+  (forall x, In x vars -> fst x = snd x) ->
+  alpha_equiv_t vars t1 t2.
+Proof.
+  unfold a_equiv_t; intros.
+  rewrite <- (app_nil_r vars).
+  rewrite alpha_equiv_t_redundant' with(v1:=vars)(v2:=nil); auto.
+Qed.
+
+Corollary a_equiv_f_expand vars f1 f2:
+  a_equiv_f f1 f2 ->
+  (forall x, In x vars -> fst x = snd x) ->
+  alpha_equiv_f vars f1 f2.
+Proof.
+  unfold a_equiv_f; intros.
+  rewrite <- (app_nil_r vars).
+  rewrite alpha_equiv_f_redundant' with (v1:=vars)(v2:=nil); auto.
+Qed.
+
+
+
+Check alpha_equiv_t_redundant.
+
+Lemma alpha_equiv_t_redundant (s: aset vsymbol) (m3 m4: amap vsymbol vsymbol) 
+  (Hnotin1: forall x, aset_mem x s -> amap_lookup m3 x = None) 
+  (Hnotin2: forall x, aset_mem x s -> amap_lookup m4 x = None)  (t1: term) (f1: formula):
+  (forall (t2: term) (m1 m2: amap vsymbol vsymbol) 
+    (Hm1: forall x, amap_lookup m1 x = Some x -> amap_mem x m2)
+    (Hm2: forall x, amap_lookup m2 x = Some x -> amap_mem x m1),
+    alpha_equiv_t (aunion m1 (aunion (mk_id_map s) m3)) (aunion m2 (aunion (mk_id_map s) m4)) t1 t2 =
+    alpha_equiv_t (aunion m1 m3) (aunion m2 m4) t1 t2) /\
+  (forall (f2: formula) (m1 m2: amap vsymbol vsymbol) 
+    (Hm1: forall x, amap_lookup m1 x = Some x -> amap_mem x m2)
+    (Hm2: forall x, amap_lookup m2 x = Some x -> amap_mem x m1),
+    alpha_equiv_f (aunion m1 (aunion (mk_id_map s) m3)) (aunion m2 (aunion (mk_id_map s) m4)) f1 f2 =
+    alpha_equiv_f (aunion m1 m3) (aunion m2 m4) f1 f2). 
+
+(**)
+
+(*
 (*Remove redundant lists - do generically so we prove once*)
 Section RemoveList.
 
@@ -7095,7 +7432,7 @@ Proof.
   specialize (Hx vs_d vs_d). subst. reflexivity.
 Qed.
 
-End AlterList. *)
+End AlterList. *)*)
 
 (*Now we come to substitution and alpha equivalence.
   To specify this, we first express that a variable occurs the
@@ -7316,13 +7653,13 @@ Qed.
 (*Similar results for specialized [amap_union]*)
 (*Note that it is very important we choose the first such variable in the union - we want to
   overwrite with newly bound pattern variables*)
-Lemma amap_union_set_infst {A B: Type} `{countable.Countable A} (m1 m2: amap A B) (x: A) (y: B):
+Lemma aunion_set_infst {A B: Type} `{countable.Countable A} (m1 m2: amap A B) (x: A) (y: B):
   amap_mem x m1 ->
-  amap_union (fun z _ => Some z) m1 (amap_set m2 x y) = amap_union (fun z _ => Some z) m1 m2.
+  aunion m1 (amap_set m2 x y) = aunion m1 m2.
 Proof.
   intros Hmem.
   apply amap_ext. intros z.
-  rewrite !amap_union_lookup.
+  rewrite !aunion_lookup.
   rewrite amap_mem_spec in Hmem.
   destruct (EqDecision0 x z); subst.
   - rewrite amap_set_lookup_same.
@@ -7330,30 +7667,29 @@ Proof.
   - rewrite amap_set_lookup_diff; auto.
 Qed.
 
-Lemma amap_union_set_not_infst {A B: Type} `{countable.Countable A} (m1 m2: amap A B) (x: A) (y: B):
+Lemma aunion_set_not_infst {A B: Type} `{countable.Countable A} (m1 m2: amap A B) (x: A) (y: B):
   ~ amap_mem x m1 ->
-  amap_union (fun z _ => Some z) m1 (amap_set m2 x y) = amap_set (amap_union (fun z _ => Some z) m1 m2) x y.
+  aunion m1 (amap_set m2 x y) = amap_set (aunion m1 m2) x y.
 Proof.
   intros Hmem.
   apply amap_ext. intros z.
-  rewrite !amap_union_lookup.
+  rewrite !aunion_lookup.
   rewrite amap_mem_spec in Hmem.
   destruct (EqDecision0 x z); subst.
   - rewrite !amap_set_lookup_same.
     destruct (amap_lookup m1 z); auto. exfalso; apply Hmem; auto.
   - rewrite !amap_set_lookup_diff; auto.
-    rewrite amap_union_lookup. auto.
+    rewrite aunion_lookup. auto.
 Qed.
 
 Lemma notin_amap_mem_union {A B: Type} `{countable.Countable A} (m1 m2: amap A B) (x: A):
   ~ amap_mem x m1 ->
   ~ amap_mem x m2 ->
-  ~ amap_mem x (amap_union (fun z _ => Some z) m1 m2).
+  ~ amap_mem x (aunion m1 m2).
 Proof.
-  rewrite !amap_mem_spec, amap_union_lookup.
-  destruct (amap_lookup m1 x); auto.
+  rewrite amap_mem_aunion_some.
+  destruct (amap_mem x m1); auto.
 Qed.
-
 
 (*Note: our theorem will probbaly be something like:
   if x not in m1 and y not in m2, then
@@ -7477,10 +7813,10 @@ Proof.
       (*Simplify LHS*)
       assert (Hinfv2: aset_mem x (pat_fv p1)) by (eapply same_in_p_fv; eauto).
       assert (Hinres1: amap_mem x res1) by (rewrite Hiff1; auto). 
-      rewrite amap_union_set_infst by auto.
+      rewrite aunion_set_infst by auto.
       (*Simplify RHS*)
       rewrite <- alpha_equiv_t_remove with (y2:=y) by auto.
-      rewrite amap_union_set_not_infst by auto.
+      rewrite aunion_set_not_infst by auto.
       (*Now we can remove the remove*)
       rewrite amap_remove_set_same, amap_remove_notin; auto.
       (*And now we just have to prove y is not in the union*)
@@ -7488,8 +7824,8 @@ Proof.
     + (*Here, use IH - by same token, x not in pat_fv p1, so not in res1 or res2
         Just need to bring amap_set forward*)
       assert (Hnotinfv': ~ aset_mem x (pat_fv p1)) by (erewrite same_in_p_fv; eauto).
-      rewrite amap_union_set_not_infst by (rewrite Hiff1; auto).
-      rewrite amap_union_set_not_infst by auto.
+      rewrite aunion_set_not_infst by (rewrite Hiff1; auto).
+      rewrite aunion_set_not_infst by auto.
       apply IHhd; auto.
       apply notin_amap_mem_union; auto.
   - (*Teps - almost same as Tlet*)
@@ -7621,14 +7957,14 @@ Proof.
     destruct (aset_mem_dec x (pat_fv p2)) as [Hinfv | Hnotinfv]; simpl; rewrite Halphap.
     + assert (Hinfv2: aset_mem x (pat_fv p1)) by (eapply same_in_p_fv; eauto).
       assert (Hinres1: amap_mem x res1) by (rewrite Hiff1; auto). 
-      rewrite amap_union_set_infst by auto.
+      rewrite aunion_set_infst by auto.
       rewrite <- alpha_equiv_f_remove with (y2:=y) by auto.
-      rewrite amap_union_set_not_infst by auto.
+      rewrite aunion_set_not_infst by auto.
       rewrite amap_remove_set_same, amap_remove_notin; auto.
       apply notin_amap_mem_union; auto.
     + assert (Hnotinfv': ~ aset_mem x (pat_fv p1)) by (erewrite same_in_p_fv; eauto).
-      rewrite amap_union_set_not_infst by (rewrite Hiff1; auto).
-      rewrite amap_union_set_not_infst by auto.
+      rewrite aunion_set_not_infst by (rewrite Hiff1; auto).
+      rewrite aunion_set_not_infst by auto.
       apply IHhd; auto.
       apply notin_amap_mem_union; auto.
 Qed.
@@ -7936,49 +8272,52 @@ Proof.
   apply alpha_equiv_sub_var_f; auto.
 Qed.
 
-(*START*)
-
 (*Congruences*)
+
+Lemma amap_singleton_set {A B: Type} `{countable.Countable A} (x: A) (y: B):
+  amap_set amap_empty x y = amap_singleton x y.
+Proof. reflexivity. Qed.
 
 Lemma alpha_tlet_congr v1 tm1 tm2 tm3 tm4:
   a_equiv_t tm1 tm3 ->
   a_equiv_t tm2 tm4 ->
   a_equiv_t (Tlet tm1 v1 tm2) (Tlet tm3 v1 tm4).
 Proof.
-  unfold a_equiv_t; simpl; intros.
-  rewrite H, eq_dec_refl; simpl_bool.
-  apply a_equiv_t_expand; simpl; auto.
-  intros x [Hx | []]; subst; auto.
+  intros Ha1 Ha2. unfold a_equiv_t; simpl.
+  rewrite eq_dec_refl. simpl. rewrite andb_true; split; auto.
+  rewrite amap_singleton_set, <- a_equiv_t_expand_single; auto.
 Qed.
 
 (*And from transitivity:*)
-Lemma alpha_convert_tlet':
+(*TODO: transitivity*)
+(*START*)
+(* Lemma alpha_convert_tlet':
 forall v1 v2 : vsymbol,
   snd v1 = snd v2 ->
   forall tm1 tm2 tm3 tm4 : term,
   ~ In v2 (tm_bnd tm4) ->
-  ~ In v2 (tm_fv tm4) ->
+  ~ aset_mem v2 (tm_fv tm4) ->
   a_equiv_t tm1 tm3 ->
   a_equiv_t tm2 tm4 ->
   a_equiv_t (Tlet tm1 v1 tm2) (Tlet tm3 v2 (sub_var_t v1 v2 tm4)).
 Proof.
-  intros.
+  intros v1 v2 Heq tm1 tm2 tm3 tm4 Hnotbnd Hnotfv Ha1 Ha2.
   eapply a_equiv_t_trans.
   2: apply alpha_convert_tlet; auto.
   apply alpha_tlet_congr; auto.
-Qed.
+Qed. *)
 
 Lemma alpha_teps_congr v f1 f2:
   a_equiv_f f1 f2 ->
   a_equiv_t (Teps f1 v) (Teps f2 v).
 Proof.
-  unfold a_equiv_f, a_equiv_t; simpl; intros.
-  rewrite eq_dec_refl; simpl.
-  apply a_equiv_f_expand; auto; simpl;
-  intros x [Hx | []]; subst; auto.
+  intros Ha. unfold a_equiv_t; simpl.
+  rewrite eq_dec_refl. simpl.
+  rewrite amap_singleton_set, <- a_equiv_f_expand_single; auto.
 Qed.
 
-Lemma alpha_convert_teps': forall v1 v2,
+(*TODO*)
+(* Lemma alpha_convert_teps': forall v1 v2,
   snd v1 = snd v2 ->
   forall f1 f2: formula,
   ~ In v2 (fmla_bnd f2) ->
@@ -7989,19 +8328,18 @@ Proof.
   intros. eapply a_equiv_t_trans.
   2: apply alpha_convert_teps; auto.
   apply alpha_teps_congr; auto.
-Qed.
+Qed. *)
 
 Lemma alpha_quant_congr q v f1 f2:
   a_equiv_f f1 f2 ->
   a_equiv_f (Fquant q v f1) (Fquant q v f2).
 Proof.
-  unfold a_equiv_f; simpl; intros.
-  rewrite !eq_dec_refl; simpl.
-  apply a_equiv_f_expand; auto; simpl;
-  intros x [Hx | []]; subst; auto.
+  intros Ha. unfold a_equiv_f; simpl.
+  rewrite !eq_dec_refl. simpl.
+  rewrite amap_singleton_set, <- a_equiv_f_expand_single; auto.
 Qed.
 
-Lemma alpha_convert_quant': forall q v1 v2,
+(* Lemma alpha_convert_quant': forall q v1 v2,
   snd v1 = snd v2 ->
   forall f1 f2: formula,
   ~ In v2 (fmla_bnd f2) ->
@@ -8013,7 +8351,7 @@ Proof.
   2: apply alpha_convert_quant; auto.
   apply alpha_quant_congr; auto.
 Qed.
-
+ *)
 Lemma alpha_tfun_congr f tys tms1 tms2:
   length tms1 = length tms2 ->
   Forall (fun x => a_equiv_t (fst x) (snd x)) (combine tms1 tms2) ->
@@ -8075,14 +8413,13 @@ Lemma alpha_flet_congr v1 tm1 tm2 f1 f2:
   a_equiv_f f1 f2 ->
   a_equiv_f (Flet tm1 v1 f1) (Flet tm2 v1 f2).
 Proof.
-  unfold a_equiv_t, a_equiv_f; simpl; intros.
-  rewrite H, eq_dec_refl; simpl_bool.
-  apply a_equiv_f_expand; simpl; auto.
-  intros x [Hx | []]; subst; auto.
+  intros Ha1 Ha2. unfold a_equiv_f; simpl.
+  rewrite eq_dec_refl. simpl. rewrite andb_true; split; auto.
+  rewrite amap_singleton_set, <- a_equiv_f_expand_single; auto.
 Qed.
 
 (*And from transitivity:*)
-Lemma alpha_convert_flet':
+(* Lemma alpha_convert_flet':
 forall v1 v2 : vsymbol,
   snd v1 = snd v2 ->
   forall tm1 tm2 f1 f2,
@@ -8096,7 +8433,7 @@ Proof.
   eapply a_equiv_f_trans.
   2: apply alpha_convert_flet; auto.
   apply alpha_flet_congr; auto.
-Qed.
+Qed. *)
 
 Lemma alpha_fif_congr f1 f2 f3 f4 f5 f6:
   a_equiv_f f1 f2 ->
@@ -8120,6 +8457,8 @@ End API.
 (*We need some iterated versions of the above free variable lemmas
   and congruence lemmas: we do terms and formulas together by
   generalizing *)
+(*TODO: see what we need here, probably for patterns so unclear*)
+(*
 Section Iter.
 
 Context {A: Type}.
@@ -8137,7 +8476,8 @@ Variable bnd_sub : forall (t: A) (x y: vsymbol),
 
 (*The iterated version of [sub_var_fv_notin]. Awkward to state so
   that we can prove term and formula versions together*)
-Lemma sub_mult_fv_notin
+(*TODO: see if we need*)
+(* Lemma sub_mult_fv_notin
   (vars: list (vsymbol * string)) (t: A)
   (Hn: NoDup (map fst vars))
   (Huniq: forall x, In x (map fst vars) -> ~ In (fst x) (map snd vars)):
@@ -8157,7 +8497,7 @@ Proof.
     + intro C; subst. contradiction.
     + destruct a; destruct v; simpl in *; intro C; inversion C; subst.
       apply (Huniq (s, v)); triv.
-Qed.
+Qed. *)
 
 Lemma sub_mult_fv_diff (vars: list (vsymbol * string)) (t: A):
   forall x, ~ In x (map fst vars) -> 
@@ -8305,7 +8645,7 @@ alpha_equiv_t_trans alpha_equiv_sub_var_t free_in_t_spec.
 Definition a_equiv_f_sub_var_fs_congr :=
 a_equiv_subs_congr _ _ sub_var_f_fv_notin sub_var_f_fv_diff _ 
 bnd_sub_var_f sub_var_f_eq _ _  alpha_f_equiv_sym alpha_equiv_f_redundant
-alpha_equiv_f_trans alpha_equiv_sub_var_f free_in_f_spec.
+alpha_equiv_f_trans alpha_equiv_sub_var_f free_in_f_spec.*)
 
 (*We give two different alpha conversion functions, with
   different properties:
@@ -8325,6 +8665,7 @@ alpha_equiv_f_trans alpha_equiv_sub_var_f free_in_f_spec.
     which require strong properties about disjointness.
     We give the first function first*)
 
+(*START (after transitivity)*)
 Section ConvertFirst.
 
 Definition mk_fun_str (l: list vsymbol) (l2: list string) :
